fairness/examples/spinlock/spinlock_sc_adequacy.v
@@ -464,20 +464,21 @@ Proof.
   set δ0 := initial_ls s0 0 I: lm_ls spinlock_model.
   (* pose conv_init := ((fun hGS => LM_init_resource 0%nat δ0): heapGS Σ LM_EM_HL -> iProp Σ). *)
 
-  unshelve eapply (simple_simulation_adequacy_terminate_ftm Σ NotStuck _ s0 _ _ ∅) =>//; cycle 1. 
+  unshelve eapply (simple_simulation_adequacy_terminate_ftm Σ NotStuck _ s0 ∅) =>//.
   - done. 
   - eapply valid_state_evolution_finitary_fairness_simple.
     intros ?. simpl.
     apply (spinlock_model_finitary s1).    
   - intros ?. iStartProof.
     rewrite /LM_init_resource.
-    iIntros (hGS). iSplitR.
-    2: { iIntros "X". iModIntro. iApply "X". }
-    iIntros "!> (Hm & ST & Hfr & Hf) !>". simpl.
+    simpl. 
+    iIntros "!> (ST & Hfr & Hf) !>". simpl.
     iAssert (|==> frag_free_roles_are ∅)%I as "-#FR".
     { rewrite /frag_free_roles_are. iApply own_unit. }
-    iSplitL. 
-    { 
+    iSplitL.
+    2: { (* TODO: make a lemma, move it to simulation_adequacy_lm *)
+      iIntros (?). iIntros "**". 
+      iApply (fupd_mask_weaken ∅); first set_solver. by iIntros "_ !>". }
     iMod "FR" as "FR". 
     iApply (program_spec _ ∅ True _ with "[] [Hf FR ST]"); eauto. 
     { iApply ActualOwnershipPartial.
@@ -487,9 +488,5 @@ Proof.
     iApply has_fuels_proper; [..| iFrame]; try done.
     rewrite /spinlock_lr. simpl.
     rewrite !gset_to_gmap_union_singleton gset_to_gmap_empty.
-    done.  }
-
-    (* TODO: make a lemma, move it to simulation_adequacy_lm *)
-    iIntros (?). iIntros "**". 
-    iApply (fupd_mask_weaken ∅); first set_solver. by iIntros "_ !>".
+    done. 
 Qed.
