fairness/heap_lang/simulation_adequacy.v
@@ -13,18 +13,17 @@ Section adequacy.
 Theorem strong_simulation_adequacy_general
     `{hPre: @heapGpreS Σ M EM} (s: stuckness) (e1 : expr) σ1 (s1: M)
     (R: execution_trace heap_lang → auxiliary_trace M → Prop)
-    (conv_init: heapGS Σ EM -> iProp Σ)
+    (p: em_init_param)
   :
   rel_finitary R →
   em_is_init_st ([e1], σ1) s1 ->
   em_valid_state_evolution_fairness {tr[ ([e1], σ1) ]} {tr[ s1 ]} ->
   (∀ `{Hinv : @heapGS Σ M EM} ,
     ⊢ (([∗ map] l ↦ v ∈ heap σ1, mapsto l (DfracOwn 1) v) ∗
-       conv_init Hinv
+       em_init_resource s1 p (em_GS0 := heap_fairnessGS)
        ={⊤}=∗
        WP e1 @ s; locale_of [] e1; ⊤ {{ _, em_thread_post 0%nat (em_GS0 := heap_fairnessGS)}} ∗
-       rel_always_holds0 R s state_interp (fun _ => em_thread_post 0%nat (em_GS0 := heap_fairnessGS)) e1 σ1 s1) ∗
-       (em_init_resource s1 (em_GS0 := heap_fairnessGS) ∗ em_msi ([e1], σ1) s1 (em_GS0 := heap_fairnessGS) ==∗ conv_init Hinv ∗ em_msi ([e1], σ1) s1 (em_GS0 := heap_fairnessGS))%I) ->
+       rel_always_holds0 R s state_interp (fun _ => em_thread_post 0%nat (em_GS0 := heap_fairnessGS)) e1 σ1 s1)) ->
   continued_simulation R (trace_singleton ([e1], σ1)) (trace_singleton s1).
 Proof.
   intros Hfin INIT VALID1 H.
@@ -40,16 +39,13 @@ Proof.
 
   set (distG := {| heap_fairnessGS := (fGS: (em_GS Σ (ExecutionModel := EM))) |}).
   (* iMod (H distG) as "Hwp". clear H. *)
-  iPoseProof (H distG) as "[Hwp CONV]". clear H.
+  iPoseProof (H distG) as "Hwp". clear H.
  
   iExists state_interp, (fun _ => em_thread_post 0%nat), fork_post.
   iSplitR.
   { unfold config_wp. iIntros "!>!>" (???????) "?". done. }
 
-  (* iApply "Hwp".  *)
-  iMod ("CONV" with "[LM_INIT MSI]") as "[LM_INIT' MSI]"; [by iFrame| ]. 
-  
-  iSpecialize ("Hwp" with "[Hσ LM_INIT']"); [by iFrame| ]. 
+  iSpecialize ("Hwp" with "[Hσ LM_INIT]"); [by iFrame| ]. 
   iDestruct "Hwp" as ">[Hwp H]". 
   iModIntro. iFrame.
 Qed.
